\documentclass{article}
\input{503macros.tex}


\begin{document}
\begin{center}
  {\LARGE CSC 503 Homework Assignment 6}\\[1pc]
  Out: September 22, 2016 \\
  Due: September 29, 2016 \\
  \unityid{aagrawa8}
\end{center}


\begin{enumerate}

\item \textbf{[15 points]} Rewrite the formula
  $[P(x,y) \land Q(x,y)] \lor [\neg R(y,x) \lor S(x)]$ in clausal form
  set notation.
  \begin{answer}
  Distributing $\lor$ across the statements will result in  $[P(x,y) \lor \neg R(y,x) \lor S(x) ] \land [Q(x,y) \lor \neg R(y,x) \lor S(x) ]   $ \\
  So in clausal form notation, it looks like,\\
  $\{\{P(x,y) , \neg R(y,x), S(x)\},$\\
  $\{Q(x,y), \neg R(y,x) , S(x)\}\}$
  \end{answer}

\item \textbf{[10 points]} Rewrite the statement
  \begin{displaymath}
    \{ \;
    \{ R(x,z), R(y,z), R(x,y) \},
    \;
    \{ R(x,y), S(y,x), \neg T(x,x) \},
    \;
    \{ T(x,y), R(y,x) \}
    \; \}
  \end{displaymath}
  so that the variables in each clause are standardized apart.
  \begin{answer}
    $\{ \{ R(x_1,z_1), R(y_1,z_1), R(x_1,y_1) \},$\\
    $\{ R(x_2,y_2), S(y_2,x_2), \neg T(x_2,x_2) \},$\\
    $\{ T(x_3,y_3), R(y_3,x_3) \}\}$
  \end{answer}

\item \textbf{[25 points]} Convert the formula
  $\forall x\ P(x,y) \iff (\forall y\ (R(x,y) \implies Q(x,y)))$ to
  negation normal form, showing the steps of the conversion.
  \begin{answer}
  Here the question can have multiple interpretations, depending on the brackets. So, I am considering $\forall x $ is associated with $P(x,y)$ not the whole statement. And $\forall y$ is outside the $(R(x,y) \implies Q(x,y))$ and when changing the implication will operate only within the brackets.\\
  $\forall x\ P(x,y) \iff (\forall y\ (R(x,y) \implies Q(x,y)))$\\
  $(\forall x\ P(x,y) \implies (\forall y\ (R(x,y) \implies Q(x,y)))) \land (\forall y\ (R(x,y) \implies Q(x,y)) \implies \forall x\ P(x,y) )$ \\
  $(\forall x\ P(x,y) \implies (\forall y\ ( \neg R(x,y) \lor Q(x,y)))) \land (\forall y\ (\neg R(x,y) \lor Q(x,y)) \implies \forall x\ P(x,y) )$ \\
  $(\neg [\forall x\ P(x,y)] \lor (\forall y\ ( \neg R(x,y) \lor Q(x,y)))) \land (\forall y\ (\neg R(x,y) \lor Q(x,y)) \implies \forall x\ P(x,y) )$ \\
  $(\exists x\ \neg P(x,y) \lor (\forall y\ ( \neg R(x,y) \lor Q(x,y)))) \land (\neg [\forall y\  (\neg R(x,y) \lor Q(x,y))] \lor \forall x\ P(x,y) )$ \\
  $(\exists x\ \neg P(x,y) \lor (\forall y\ ( \neg R(x,y) \lor Q(x,y)))) \land (\exists y\ \neg (\neg R(x,y) \lor Q(x,y)) \lor \forall x\ P(x,y) )$ \\
 $(\exists x\ \neg P(x,y) \lor (\forall y\ ( \neg R(x,y) \lor Q(x,y)))) \land (\exists y\ (\neg \neg R(x,y) \land \neg Q(x,y)) \lor \forall x\ P(x,y) )$ \\ 
 $(\exists x\ \neg P(x,y) \lor (\forall y\ ( \neg R(x,y) \lor Q(x,y)))) \land (\exists y\ ( R(x,y) \land \neg Q(x,y)) \lor \forall x\ P(x,y) )$ \\
 \end{answer}

\item \textbf{[25 points]} Convert the formula
  $\exists x\ [(\forall y\ P(x,y)) \implies (\exists z\ Q(x,z))]$ to
  prenex normal form, showing the steps of the conversion.
    \begin{answer}
    $\exists x\ [(\forall y\ P(x,y)) \implies (\exists z\ Q(x,z))]$\\
    $\exists x \exists y \ [\ P(x,y) \implies (\exists z\ Q(x,z))]$\\
    $\exists x \exists y \exists z \ [\ P(x,y) \implies \ Q(x,z)]$\\
  \end{answer}

\item \textbf{[25 points]} Convert
  $\exists x\ \forall y\ ([P(x,y) \land (\forall z\ Q(y,z))] \implies
  [\exists u\ \exists v\ (P(x,v) \land R(y,v))])$ to the language of
  resolution, showing the conversion steps.  That is, first convert to
  NNF, then Skolemize, then convert to PNF, then convert to CNF, then
  convert to an open formula, and finally to clausal set notatation
  standardized apart.
  \begin{answer}
  $\exists x\ \forall y\ ([P(x,y) \land (\forall z\ Q(y,z))] \implies [\exists u\ \exists v\ (P(x,v) \land R(y,v))])$\\
  Converting to NNF form first,\\
  $\exists x\ \forall y\ (\neg [P(x,y) \land (\forall z\ Q(y,z))] \lor [\exists u\ \exists v\ (P(x,v) \land R(y,v))])$\\
  $\exists x\ \forall y\ ( [\neg P(x,y) \lor \neg (\forall z\ Q(y,z))] \lor [\exists u\ \exists v\ (P(x,v) \land R(y,v))])$\\
  $\exists x\ \forall y\ ( [\neg P(x,y) \lor (\exists z\ \neg Q(y,z))] \lor [\exists u\ \exists v\ (P(x,v) \land R(y,v))])$\\
  Skolemize the above statement,\\
  $\exists x\ \forall y \exists z \exists u \exists v \ ( [\neg P(x,y) \lor \ \neg Q(y,z)] \lor [\  P(x,v) \land R(y,v)])$\\
  Now replacing z by function f(y), and v by g(y).\\
  $\exists x\ \forall y \ ( [\neg P(x,y) \lor \neg Q(y,f(y))] \lor [\  P(x,g(y)) \land R(y,g(y))])$\\
  Now, for $\exists x$, replacing it with a constant 'c'. This will also bring it to PNF form\\
  $\forall y \ ( [\neg P(c,y) \lor \neg Q(y,f(y))] \lor [\  P(c,g(y)) \land R(y,g(y))])$\\
  Converting to CNF form,\\
  $\forall y \ ( [\neg P(c,y) \lor \neg Q(y,f(y)) \lor P(c,g(y))] \land [\ \neg P(c,y) \lor \neg Q(y,f(y)) \lor  R(y,g(y))])$\\
  Converting to open formula,\\
    $ [\neg P(c,y) \lor \neg Q(y,f(y)) \lor P(c,g(y))] \land [\ \neg P(c,y) \lor \neg Q(y,f(y)) \lor  R(y,g(y))]$\\
  Converting to Clausal set formula,\\
    $ \{\{\neg P(c,y), \neg Q(y,f(y)), P(c,g(y))\},$ \\
    $\{\neg P(c,y), \neg Q(y,f(y)), R(y,g(y))\}\}$\\
    Standardized form\\
    $ \{\{\neg P(c,y_1), \neg Q(y_1,f(y_1)), P(c,g(y_1))\},$ \\
    $\{\neg P(c,y_2), \neg Q(y_2,f(y_2)), R(y_2,g(y_2))\}\}$\\
  \end{answer}

\end{enumerate}

\end{document}
